TestModels/dafny-dependencies/StandardLibrary/src/Actions/Actions.dfy
@@ -1,0 +1,708 @@
+
+include "../../../libraries/src/Wrappers.dfy"
+
+include "../Frames.dfy"
+include "GenericAction.dfy"
+include "DecreasesClauses.dfy"
+include "../DynamicArray.dfy"
+include "../Seq.dfy"
+
+module {:options "--function-syntax:4"} Std.Actions {
+
+  import opened Wrappers
+  import opened Frames
+  import opened GenericActions
+  import opened Termination
+  import opened DynamicArray
+  import Seq
+
+  // TODO: Documentation, especially overall design
+  trait {:termination false} Action<T, R> extends GenericAction<T, R>, Validatable {
+
+    ghost var history: seq<(T, R)>
+
+    ghost predicate Valid()
+      reads this, Repr
+      ensures Valid() ==> this in Repr
+      ensures Valid() ==> CanProduce(history)
+      decreases height, 0
+
+    // KEY DESIGN POINT: these predicates specifically avoid reading the current
+    // state of the action.
+    // That's so extrisnic properties of an action do NOT depend on their current state.
+    // This is key to ensure that you can prove properties of a given action that
+    // will continue to hold as the Dafny heap changes.
+    // This approach works because Dafny understands that for a given object,
+    // the implementation of CanConsume/CanProduce cannot change over time.
+    //
+    // The downside is that these are then forced to use quantifiers
+    // to talk about all possible states of an action.
+    // The solution is the trait proof pattern,
+    // where a trait is passed around with an abstract lemma
+    // that can be invoked on the otherwise quantified state as needed.
+
+    // TODO: Necessary but not sufficient that:
+    // CanConsume(history, nextIn) ==> exists nextOut :: CanProduce(history + [(nextIn, nextOut)])
+    // Does that need to be explicitly part of the spec?
+    ghost predicate CanConsume(history: seq<(T, R)>, next: T)
+      requires CanProduce(history)
+      decreases height
+
+    ghost predicate CanProduce(history: seq<(T, R)>)
+      decreases height
+
+    ghost predicate Requires(t: T)
+      reads Reads(t) 
+    {
+      && Valid()
+      && CanConsume(history, t)
+    }
+    ghost function Reads(t: T): set<object> 
+      reads this
+      ensures this in Reads(t)
+    {
+      {this} + Repr
+    }
+    ghost function Modifies(t: T): set<object> 
+      reads Reads(t)
+    {
+      Repr
+    }
+    ghost function Decreases(t: T): TerminationMetric 
+      reads Reads(t)
+    {
+      NatTerminationMetric(height)
+    }
+    twostate predicate Ensures(t: T, new r: R) 
+      reads Reads(t)
+    {
+      && Valid()
+      && history == old(history) + [(t, r)]
+      && fresh(Repr - old(Repr))
+    }
+
+    // Possibly optimized extensions
+
+    // // Equivalent to DefaultRepeatUntil below, but may be implemented more efficiently.
+    // method RepeatUntil(t: T, stop: R -> bool)
+    //   requires Valid()
+    //   requires EventuallyStops(this, t, stop)
+    //   requires forall i <- Consumed() :: i == t
+    //   // reads Reads(t)
+    //   modifies Repr
+    //   ensures Valid()
+    //   //ensures history == old(history) + (n copies of t)/(n - 1 not stop values + stop)
+
+    // Helpers
+
+    ghost method Update(t: T, r: R)
+      modifies `history
+      ensures history == old(history) + [(t, r)]
+    {
+      history := history + [(t, r)];
+    }
+
+    ghost function Consumed(): seq<T> 
+      reads this
+    {
+      Inputs(history)
+    }
+
+    ghost function Produced(): seq<R> 
+      reads this
+    {
+      Outputs(history)
+    }
+  }
+
+  // method DefaultRepeatUntil<T, R>(a: Action<T, R>, t: T, stop: R -> bool) 
+  //   requires a.Valid()
+  //   requires EventuallyStops(a, t, stop)
+  //   requires forall i <- a.Consumed() :: i == t
+  //   // reads a.Repr
+  //   modifies a.Repr
+  //   ensures a.Valid()
+  // {
+  //   // TODO: loops need to support reads clauses as well!
+
+  //   while (true) 
+  //     modifies a.Repr
+  //     invariant a.Valid()
+  //     invariant fresh(a.Repr - old(a.Repr))
+  //     invariant forall i <- a.Consumed() :: i == t
+  //     decreases InvokeUntilTerminationMetric(a, t, stop)
+  //   {
+  //     label beforeInvoke:
+  //     assert a.Valid();
+  //     var next := a.Invoke(t);
+  //     var nextV := next;
+  //     if stop(nextV) {
+  //       break;
+  //     }
+  //     InvokeUntilTerminationMetricDecreased@beforeInvoke(a, t, stop, next);
+  //   }
+  // }
+
+  // Dependencies stolen from DafnyStandardLibraries
+  
+  function Max(a: int, b: int): int
+  {
+    if a < b
+    then b
+    else a
+  }
+
+  function Min(a: int, b: int): int
+  {
+    if a < b
+    then a
+    else b
+  }
+
+  // Common action invariants
+
+  function Inputs<T, R>(history: seq<(T, R)>): seq<T> {
+    Seq.Map((e: (T, R)) => e.0, history)
+  }
+
+  function Outputs<T, R>(history: seq<(T, R)>): seq<R> {
+    Seq.Map((e: (T, R)) => e.1, history)
+  }
+
+  trait ConsumesAllProof<T, R> {
+    function Action(): Action<T, R>
+
+    lemma Proof(history: seq<(T, R)>, next: T) 
+      requires Action().CanProduce(history)
+      ensures Action().CanConsume(history, next)
+  }
+
+  method CallOnce<R>(a: Action<int, R>, ghost p: ConsumesAllProof<int, R>) 
+    requires a.Valid()
+    requires p.Action() == a
+    modifies a, a.Repr
+  {
+    p.Proof(a.history, 42);
+    var x := a.Invoke(42);
+  }
+
+  method Main() {
+    var a := new ArrayAggregator<int>();
+    ghost var proof := new ArrayAggregatorConsumesAnythingProof(a);
+    CallOnce(a, proof);
+  }
+
+  ghost predicate OnlyProduces<T, R>(i: Action<T, R>, history: seq<(T, R)>, c: R) 
+  {
+    i.CanProduce(history) <==> forall e <- history :: e.1 == c
+  }
+
+  ghost predicate Terminated<T>(s: seq<T>, stop: T -> bool, n: nat) {
+    forall i | 0 <= i < |s| :: n <= i <==> stop(s[i])
+  }
+
+  lemma TerminatedDistributes<T>(left: seq<T>, right: seq<T>, stop: T -> bool, n: nat)
+    requires Terminated(left, stop, |left|)
+    requires Terminated(right, stop, n)
+    ensures Terminated(left + right, stop, |left| + n)
+  {}
+
+  lemma TerminatedUndistributes<T>(left: seq<T>, right: seq<T>, stop: T -> bool, n: nat)
+    requires Terminated(left + right, stop, n)
+    ensures Terminated(left, stop, n)
+    ensures Terminated(right, stop, Max(0, n - |left|))
+  {
+    assert forall i | 0 <= i < |left| :: left[i] == (left + right)[i];
+    assert forall i | 0 <= i < |right| :: right[i] == (left + right)[i + |left|];
+  }
+
+  // TODO: generalize to "EventuallyProducesSequence"?
+  // ghost predicate ProducesTerminatedBy<T, R>(i: Action<T, R>, stop: R -> bool, limit: nat) {
+  //   forall history: seq<(T, R)> | i.CanProduce(history) 
+  //     :: exists n: nat | n <= limit :: Terminated(Outputs(history), stop, n)
+  // }
+
+  // Class of actions whose precondition doesn't depend on history (probably needs a better name)
+  // ghost predicate ContextFree<T, R>(a: Action<T, R>, p: T -> bool) {
+  //   forall history, next | a.CanProduce(history)
+  //     :: a.CanConsume(history, next) <==> p(next)
+  // }
+
+  trait ProducesTerminatedProof<T, R> {
+
+    function Action(): Action<T, R>
+    function FixedInput(): T
+    function StopFn(): R -> bool
+    function Limit(): nat
+
+    lemma Proof(history: seq<(T, R)>) 
+      requires Action().CanProduce(history) 
+      requires (forall i <- Inputs(history) :: i == FixedInput())
+      ensures exists n: nat | n <= Limit() :: Terminated(Outputs(history), StopFn(), n)
+  }
+
+  trait EventuallyStopsProof<T, R> {
+
+    function Action(): Action<T, R>
+
+    lemma Proof(history: seq<(T, R)>, input: T, stop: R -> bool, limit: nat) 
+      requires Action().CanProduce(history) 
+      requires (forall i <- Inputs(history) :: i == input)
+      ensures exists n: nat | n <= limit :: Terminated(Outputs(history), stop, n)
+  }
+
+  // ghost predicate ProducesTerminated<T, R>(e: Action<T, R>, input: T, stop: R -> bool, limit: nat) {
+  //   forall history: seq<(T, R)> 
+  //     | && e.CanProduce(history) 
+  //       && (forall i <- Inputs(history) :: i == input)
+  //     ::
+  //       exists n: nat | n <= limit :: Terminated(Outputs(history), stop, n)
+  // }
+
+  // ghost predicate EventuallyStops<T, R>(a: Action<T, R>, input: T, stop: R -> bool) {
+  //   && ConsumesAll(a, input)
+  //   && exists limit: nat :: ProducesTerminated(a, input, stop, limit)
+  // }
+
+  // ghost function InvokeUntilBound<T, R>(a: Action<T, R>, input: T, stop: R -> bool): (limit: nat)
+  //   requires EventuallyStops(a, input, stop)
+  //   ensures ProducesTerminated(a, input, stop, limit)
+  // {
+  //   var limit: nat :| ProducesTerminated(a, input, stop, limit);
+  //   limit
+  // }
+
+  // ghost function InvokeUntilTerminationMetric<T, R>(a: Action<T, R>, input: T, stop: R -> bool): nat
+  //   requires a.Valid()
+  //   requires EventuallyStops(a, input, stop)
+  //   requires forall i <- a.Consumed() :: i == input
+  //   reads a.Repr
+  // {
+  //   var limit := InvokeUntilBound(a, input, stop);
+  //   var n: nat :| n <= limit && Terminated(a.Produced(), stop, n);
+  //   TerminatedDefinesNonTerminalCount(a.Produced(), stop, n);
+  //   limit - NonTerminalCount(a.Produced(), stop)
+  // }
+
+  function NonTerminalCount<T>(produced: seq<T>, stop: T -> bool): nat {
+    if |produced| == 0 || stop(produced[0]) then
+      0
+    else
+      1 + NonTerminalCount(produced[1..], stop)
+  }
+
+  lemma TerminatedDefinesNonTerminalCount<T>(s: seq<T>, stop: T -> bool, n: nat) 
+    requires Terminated(s, stop, n)
+    ensures NonTerminalCount(s, stop) == Min(|s|, n)
+  {
+    if n == 0 || |s| == 0 {
+    } else {
+      if stop(s[0]) {
+      } else {
+        assert 1 <= NonTerminalCount(s, stop);
+        TerminatedDefinesNonTerminalCount(s[1..], stop, n - 1);
+      }
+    }
+  }
+
+  // twostate lemma InvokeUntilTerminationMetricDecreased<T, R>(a: Action<T, R>, input: T, stop: R -> bool, new nextProduced: R)
+  //   requires old(a.Valid())
+  //   requires a.Valid()
+  //   requires EventuallyStops(a, input, stop)
+  //   requires forall i <- old(a.Consumed()) :: i == input
+  //   requires a.Consumed() == old(a.Consumed()) + [input]
+  //   requires a.Produced() == old(a.Produced()) + [nextProduced]
+  //   requires !stop(nextProduced)
+  //   ensures InvokeUntilTerminationMetric(a, input, stop) < old(InvokeUntilTerminationMetric(a, input, stop))
+  // {
+  //   var before := old(a.Produced());
+  //   var after := a.Produced();
+  //   var limit := InvokeUntilBound(a, input, stop);
+  //   var n: nat :| n <= limit && Terminated(before, stop, n);
+  //   var m: nat :| m <= limit && Terminated(after, stop, m);
+  //   if n < |before| {
+  //     assert stop(before[|before| - 1]);
+  //     assert !stop(a.Produced()[|a.Produced()| - 1]);
+  //     assert |a.Produced()| <= m;
+  //     assert !stop(a.Produced()[|before| - 1]);
+  //     assert false;
+  //   } else {
+  //     TerminatedDefinesNonTerminalCount(before, stop, n);
+  //     assert NonTerminalCount(before, stop) <= n;
+  //     TerminatedDistributes(before, [nextProduced], stop, 1);
+  //     assert Terminated(after, stop, |after|);
+  //     TerminatedDefinesNonTerminalCount(after, stop, |after|);
+  //   }
+  // }
+
+  // Aggregators
+
+  // TODO: Names need improvement
+  type IAggregator<T> = Action<T, ()>
+  // type Aggregator<T> = a: Action<T, bool> | exists limit: nat :: ProducesTerminatedBy(a, r => !r, limit) witness *
+  type Accumulator<T> = Action<Option<T>, ()> // | exists limit :: ConsumesTerminatedBy(a, None, limit) witness *
+
+  class ArrayAggregator<T> extends Action<T, ()> {
+
+    var storage: DynamicArray<T>
+
+    ghost predicate Valid() 
+      reads this, Repr 
+      ensures Valid() ==> this in Repr 
+      ensures Valid() ==> 
+        && CanProduce(history)
+      decreases height, 0
+    {
+      && this in Repr
+      && storage in Repr
+      && this !in storage.Repr
+      && storage.Repr <= Repr
+      && storage.Valid?()
+      && Consumed() == storage.items
+    }
+
+    constructor() 
+      ensures Valid()
+      ensures fresh(Repr - {this})
+      ensures history == []
+    {
+      var a := new DynamicArray();
+
+      history := [];
+      height := 1;
+      Repr := {this} + {a} + a.Repr;
+      this.storage := a;
+    }
+
+    ghost predicate CanConsume(history: seq<(T, ())>, next: T)
+      decreases height
+    {
+      true
+    }
+    ghost predicate CanProduce(history: seq<(T, ())>)
+      decreases height
+    {
+      true
+    }
+
+    method Invoke(t: T) returns (r: ()) 
+      requires Requires(t)
+      modifies Modifies(t)
+      decreases Decreases(t).Ordinal()
+      ensures Ensures(t, r)
+    {
+      assert Consumed() == storage.items;
+      storage.Push(t);
+
+      r := ();
+      Update(t, r);
+      Repr := {this} + {storage} + storage.Repr;
+      assert Consumed() == old(Consumed()) + [t];
+      assert Valid();
+    }
+
+    // method RepeatUntil(t: T, stop: (()) -> bool)
+    //   requires Valid()
+    //   requires EventuallyStops(this, t, stop)
+    //   requires forall i <- Consumed() :: i == t
+    //   // reads Reads(t)
+    //   modifies Repr
+    //   ensures Valid()
+    // {
+    //   DefaultRepeatUntil(this, t, stop);
+    // }
+  }
+
+  class ArrayAggregatorConsumesAnythingProof<T> extends ConsumesAllProof<T, ()> {
+
+    const a: ArrayAggregator<T>
+
+    ghost constructor(a: ArrayAggregator<T>) 
+      ensures this.a == a
+    {
+      this.a := a;
+    }
+
+    function Action(): Action<T, ()> {
+      a
+    }
+
+    lemma Proof(history: seq<(T, ())>, next: T) 
+      requires Action().CanProduce(history)
+      ensures Action().CanConsume(history, next) 
+    {
+    }
+  }
+
+  method {:rlimit 0} AggregatorExample() {
+    var a: ArrayAggregator<nat> := new ArrayAggregator();
+    var _ := a.Invoke(1);
+    var _ := a.Invoke(2);
+    var _ := a.Invoke(3);
+    var _ := a.Invoke(4);
+    var _ := a.Invoke(5);
+    var _ := a.Invoke(6);
+    assert a.Consumed() == [1, 2, 3, 4, 5, 6];
+    assert a.storage.items == [1, 2, 3, 4, 5, 6];
+  }
+
+  class FunctionalEnumerator<S, T> extends Action<(), Option<T>> {
+
+    const stepFn: S -> Option<(S, T)>
+    var state: S
+
+    ghost predicate Valid() 
+      reads this, Repr 
+      ensures Valid() ==> this in Repr 
+      ensures Valid() ==> CanProduce(history)
+      decreases height, 0
+    {
+      this in Repr
+    }
+
+    constructor(state: S, stepFn: S -> Option<(S, T)>) {
+      this.state := state;
+      this.stepFn := stepFn;
+    }
+
+    ghost predicate CanConsume(history: seq<((), Option<T>)>, next: ())
+      decreases height
+    {
+      true
+    }
+    ghost predicate CanProduce(history: seq<((), Option<T>)>)
+      decreases height
+    {
+      true
+    }
+
+    method Invoke(t: ()) returns (r: Option<T>) 
+      requires Requires(t)
+      modifies Modifies(t)
+      decreases Decreases(t).Ordinal()
+      ensures Ensures(t, r)
+    {
+      var next := stepFn(state);
+      match next {
+        case Some(result) => {
+          var (newState, result') := result;
+          state := newState;
+          r := Some(result');
+        }
+        case None => {
+          r := None;
+        }
+      }
+      Update(t, r);
+    }
+
+    // method RepeatUntil(t: (), stop: Option<T> -> bool)
+    //   requires Valid()
+    //   requires EventuallyStops(this, t, stop)
+    //   requires forall i <- Consumed() :: i == t
+    //   // reads Reads(t)
+    //   modifies Repr
+    //   ensures Valid()
+    // {
+    //   DefaultRepeatUntil(this, t, stop);
+    // }
+  }
+
+  class Box {
+    const i: nat
+
+    constructor(i: nat) 
+      ensures this.i == i
+    {
+      this.i := i;
+    }
+  }
+
+  function SeqRange(n: nat): seq<nat> {
+    seq(n, i => i)
+  }
+
+  lemma SeqRangeIncr(prefix: seq<nat>, n: nat)
+    requires prefix == SeqRange(n)
+    ensures prefix + [n] == SeqRange(n + 1) 
+  {}
+
+  class BoxEnumerator extends Action<(), Box> {
+
+    var nextValue: nat
+
+    ghost predicate Valid() 
+      reads this, Repr 
+      ensures Valid() ==> this in Repr 
+      ensures Valid() ==> CanProduce(history)
+      decreases height, 0
+    {
+      && this in Repr
+      && CanProduce(history)
+      && nextValue == |history|
+    }
+
+    constructor() 
+      ensures Valid()
+      ensures fresh(Repr)
+      ensures history == []
+    {
+      nextValue := 0;
+      history := [];
+      Repr := {this};
+      height := 1;
+    }
+
+    ghost predicate CanConsume(history: seq<((), Box)>, next: ())
+      decreases height
+    {
+      true
+    }
+    ghost predicate CanProduce(history: seq<((), Box)>)
+      decreases height
+    {
+      Seq.Map((b: Box) => b.i, Outputs(history)) == SeqRange(|history|)
+    }
+
+    method Invoke(t: ()) returns (r: Box) 
+      requires Requires(t)
+      modifies Modifies(t)
+      decreases Decreases(t).Ordinal()
+      ensures Ensures(t, r)
+    {
+      ghost var producedBefore := Produced();
+
+      r := new Box(nextValue);
+      Update(t, r);
+      Repr := {this};
+      nextValue := nextValue + 1;
+
+      SeqRangeIncr(Seq.Map((b: Box) => b.i, producedBefore), |producedBefore|);
+      assert Valid();
+    }
+
+    // method RepeatUntil(t: (), stop: Box -> bool)
+    //   requires Valid()
+    //   requires EventuallyStops(this, t, stop)
+    //   requires forall i <- Consumed() :: i == t
+    //   // reads Reads(t)
+    //   modifies Repr
+    //   ensures Valid()
+    // {
+    //   DefaultRepeatUntil(this, t, stop);
+    // }
+  }
+
+  method {:rlimit 0} BoxEnumeratorExample() {
+    var enum: BoxEnumerator := new BoxEnumerator();
+    assert |enum.Produced()| == 0;
+    var a := enum.Invoke(());
+
+    assert enum.Produced() == [a];
+    assert Seq.Map((b: Box) => b.i, enum.Produced()) == SeqRange(1) == [0];
+    // assert a.i == 0;
+    
+    // var b := enum.Invoke(());
+    // var c := enum.Invoke(());
+    // var d := enum.Invoke(());
+    // var e := enum.Invoke(());
+
+  }
+
+  // Other primitives/examples todo:
+  //  * Promise-like single-use Action<T, ()> to capture a value for reading later
+  //  * datatype/codatatype-based enumerations
+  //  * Eliminate all the (!new) restrictions - look into "older" parameters?
+  //    * How to state the invariant that a constructor as an action creates a new object every time?
+  //      * Lemma that takes produced as input, instead of forall produced?
+  //  * Enumerable ==> defines e.Enumerator()
+  //    * BUT can have infinite containers, probably need IEnumerable as well? (different T for the Action)
+  //  * Expressing that an Action "Eventually produces something" (look at how VMC models this for randomness)
+  //    * IsEnumerator(a) == "a eventually produces None" && "a then only produces None"
+  //    * Build on that to make CrossProduct(enumerable1, enumerable2)
+  //  * Example of adapting an iterator
+  //  * Example of enumerating all possible values of a type (for test generation)
+  //    * Needs to handle infinite types too, hence needs the "eventually produces something" concept
+  //  * Document: useful pattern to add an Action<Command, Result> facade
+  //        to a set of methods that participate in a protocol.
+  //        Then you have a history that ties the behavior
+  //        of the methods together,
+  //        supporting constraints on the order of calls etc.
+
+
+  // TODO
+  // class Folder<T, R> extends Action<T, bool> {
+
+  //   const f: (R, T) -> R
+  //   var value: R
+
+  //   constructor(init: R, f: (R, T) -> R) {
+  //     this.f := f;
+  //     this.value := init;
+  //   }
+
+  //   method {:verify false} Call(t: T) returns (success: bool) {
+  //     value := f(value, t);
+  //     return success;
+  //   }
+
+  // }
+
+  // TODO: This is also a Folder([], (x, y) => x + [y])
+  class Collector<T, TV(!new)> extends Action<Option<T>, ()> {
+
+    var values: seq<T>
+
+    constructor() {
+      values := [];
+    }
+
+    ghost predicate Valid() 
+      reads this, Repr 
+      ensures Valid() ==> this in Repr 
+      ensures Valid() ==> CanProduce(history)
+      decreases height, 0
+    {
+      this in Repr 
+    }
+
+    ghost predicate CanConsume(history: seq<(Option<T>, ())>, next: Option<T>)
+      requires CanProduce(history)
+      decreases height
+    {
+      true
+    }
+
+    ghost predicate CanProduce(history: seq<(Option<T>, ())>)
+      decreases height
+    {
+      true
+    }
+
+    method {:verify false} Invoke(t: Option<T>) returns (nothing: ()) {
+      if t.Some? {
+        values := values + [t.value];
+      }
+    }
+
+    // method RepeatUntil(t: Option<T>, stop: (()) -> bool)
+    //   requires Valid()
+    //   requires EventuallyStops(this, t, stop)
+    //   requires forall i <- Consumed() :: i == t
+    //   // reads Reads(t)
+    //   modifies Repr
+    //   ensures Valid()
+    // {
+    //   DefaultRepeatUntil(this, t, stop);
+    // }
+
+    method {:verify false} Pop() returns (t: T) 
+      requires 0 < |values|
+    {
+      t := values[0];
+      values := values[1..];
+    }
+
+  }
+
+}
