TestModels/dafny-dependencies/StandardLibrary/src/Actions/Enumerators.dfy
@@ -1,0 +1,197 @@
+
+include "Actions.dfy"
+
+module {:options "--function-syntax:4"} Std.Enumerators {
+
+  import opened Actions
+  import opened Wrappers
+
+  type IEnumerator<T> = Action<(), T>
+  type Enumerator<T, TV(!new)> = a: Action<(), Option<T>> | IsEnumerator(a) witness *
+  
+  ghost predicate IsEnumerator<T, TV(!new)>(a: Action<(), Option<T>>) {
+    EventuallyStops(a, (), (r: Option<TV>) => r.None?)
+  }
+
+  function Enumerated<T>(produced: seq<Option<T>>): seq<T> {
+    if |produced| == 0 || produced[0].None? then
+      []
+    else
+      [produced[0].value] + Enumerated(produced[1..])
+  }
+
+  class SeqEnumerator<T, TV(!new)> extends Action<(), Option<T>> {
+
+    const elements: seq<T>
+    var index: nat
+
+    constructor(elements: seq<T>) 
+      ensures Valid()
+    {
+      this.elements := elements;
+      this.index := 0;
+
+      Repr := {this};
+      inputF := x => x;
+    }
+
+    ghost predicate Valid() 
+      reads this, Repr 
+      ensures Valid() ==> this in Repr 
+      ensures Valid() ==> CanProduce(history)
+      decreases height, 0
+    {
+      && this in Repr
+      && inputF == x => x
+    }
+    
+    ghost predicate CanConsume(history: seq<((), Option<TV>)>, next: ())
+      requires CanProduce(history)
+      decreases height
+    {
+      true
+    }
+
+    ghost predicate CanProduce(history: seq<((), Option<TV>)>)
+      decreases height
+    {
+      var index := |history|;
+      var values := Min(index, |elements|);
+      var nones := index - values;
+      && (forall i <- Inputs(history) :: i == ())
+      && Outputs(history) == Seq.Map(x => outputF(Some(x)), elements[..values]) + Seq.Repeat(None, nones)
+    }
+
+    method Invoke(t: ()) returns (value: Option<T>) 
+      requires Requires(t)
+      modifies Modifies(t)
+      decreases Decreases(t).Ordinal()
+      ensures Ensures(t, value)
+    {
+      if |elements| <= index {
+        value := None;
+      } else {
+        value := Some(elements[index]);
+        index := index + 1;
+      }
+      Update((), value);
+      assert Valid();
+    }
+
+    method RepeatUntil(t: (), stop: Option<TV> -> bool)
+      requires Valid()
+      requires EventuallyStops(this, t, stop)
+      requires forall i <- Consumed() :: i == inputF(t)
+      // reads Reads(t)
+      modifies Repr
+      ensures Valid()
+    {
+      DefaultRepeatUntil(this, t, stop);
+    }
+
+    lemma ThisIsEnumerator() 
+      ensures IsEnumerator(this)
+    {
+      assert forall history | CanProduce(history) :: CanConsume(history,inputF(()));
+      var stop := (r: Option<TV>) => r.None?;
+      forall history: seq<((), Option<TV>)> 
+      | && CanProduce(history) 
+        && (forall i <- Inputs(history) :: i == inputF(())) 
+        ensures exists n: nat | n <= |elements| :: Terminated(Outputs(history), stop, n)
+      {
+        var outputs := Outputs(history);
+        assert forall x :: stop(x) == x.None?;
+        var index := |history|;
+        var values := Min(index, |elements|);
+        var nones := index - values;
+        assert outputs == Seq.Map(x => outputF(Some(x)), elements[..values]) + Seq.Repeat(None, nones);
+        assert forall i | 0 <= i < |outputs| :: i < values <==> outputs[i].None?;
+        assert Terminated(Outputs(history), stop, |elements|);
+      }
+      assert ProducesTerminated(this, (), (x: Option<TV>) => x.None?, |elements|);
+    }
+
+  }
+
+  trait {:termination false} Pipeline<U, UV(!new), T, TV(!new)> extends Action<(), Option<T>> {
+    
+
+    const upstream: Enumerator<U, UV>
+    const buffer: Collector<T, TV>
+
+    method {:verify false} Invoke(nothing: ()) returns (t: Option<T>) {
+      while (|buffer.values| == 0) {
+        var u := upstream.Invoke(());
+        Process(u, buffer);
+
+        if u.None? {
+          break;
+        }
+      }
+
+      if 0 < |buffer.values| {
+        var next := buffer.Pop();
+        return Some(next);
+      } else {
+        return None;
+      }
+    }
+
+    // method {:verify false} ForEach(a: Accumulator<T, TV>)
+    // {
+    //   var a' := new PipelineProcessor(this, a);
+    //   upstream.ForEach(a');
+    // }
+
+    method Process(u: Option<U>, a: Accumulator<T, TV>)
+
+  }
+
+  class PipelineProcessor<U, UV(!new), T, TV(!new)> extends Action<Option<U>, ()> {
+
+    const pipeline: Pipeline<U, UV, T, TV>
+    const accumulator: Accumulator<T, TV>
+
+    constructor(pipeline: Pipeline<U, UV, T, TV>, accumulator: Accumulator<T, TV>) {
+      this.pipeline := pipeline;
+      this.accumulator := accumulator;
+    }
+
+    ghost predicate Valid() 
+      reads this, Repr 
+      ensures Valid() ==> this in Repr 
+      ensures Valid() ==> CanProduce(history)
+      decreases height, 0
+    {
+      this in Repr 
+    }
+
+    ghost predicate CanConsume(history: seq<(Option<UV>, ())>, next: Option<UV>)
+      requires CanProduce(history)
+      decreases height
+    {
+      true
+    }
+
+    ghost predicate CanProduce(history: seq<(Option<UV>, ())>)
+      decreases height
+    {
+      true
+    }
+
+    method {:verify false} Invoke(u: Option<U>) returns (nothing: ()) {
+      pipeline.Process(u, accumulator);
+    }
+
+    method RepeatUntil(t: Option<U>, stop: (()) -> bool)
+      requires Valid()
+      requires EventuallyStops(this, t, stop)
+      requires forall i <- Consumed() :: i == inputF(t)
+      // reads Reads(t)
+      modifies Repr
+      ensures Valid()
+    {
+      DefaultRepeatUntil(this, t, stop);
+    }
+  }
+}
